src/Prefix.v
@@ -1,0 +1,146 @@
+Require Import Coq.Lists.List.
+Import ListNotations.
+
+Require Import Coq.Relations.Relation_Definitions.
+
+Set Implicit Arguments.
+
+Fixpoint prefix A (xs ys:list A) :=
+  match xs,ys with
+  | [],_ => True
+  | x::xs,y::ys => x=y /\ prefix xs ys
+  | _,[] => False end.
+
+Lemma prefix_order A : order _ (@prefix A).
+Proof.
+  split.
+  - intros x; induction x; firstorder.
+  - intros x.
+    induction x; intros y; destruct y; try easy.
+    intros z H1 H2.
+    destruct z; simpl in *; try easy.
+    destruct H1 as (E1,H1), H2 as (E2,H2).
+    split.
+    + now rewrite E1.
+    + now apply IHx with y.
+  - unfold antisymmetric.
+    intros x; induction x; simpl in *.
+    + intros y; destruct y; easy.
+    + intros y Hy; destruct y; try easy; simpl in *.
+      intros H.
+      destruct Hy as (Ey,Hy).
+      f_equal; try easy.
+      now apply IHx.
+Qed.
+
+Lemma prefix_app A (xs ys : list A) : prefix xs (xs++ys).
+Proof. induction xs; firstorder. Qed.
+
+Lemma prefix_napp A (xs ys : list A) : ys <> [] -> ~ (prefix (xs++ys) xs).
+Proof.
+  intros H.
+  apply exists_last in H; destruct H as (H1,(zs,H2)).
+  rewrite H2.
+  intros Z.
+  induction xs; simpl in *.
+  - destruct (H1 ++ [zs]) eqn:eq; try easy.
+    now destruct H1.
+  - firstorder.
+Qed.
+
+Lemma prefix_ex A (xs ys:list A) : prefix xs ys -> exists zs, ys= xs ++ zs.
+Proof.
+  revert ys.
+  induction xs; intros ys H.
+  - exists ys; intuition.
+  - destruct ys; simpl in H; try easy.
+    destruct H as (E,H).
+    apply IHxs in H.
+    destruct H as (zs,H).
+    exists zs.
+    now rewrite E, <- app_comm_cons; f_equal.
+Qed.
+
+Lemma neq_extend A (xs ys:list A) a : a::xs <> a::ys -> xs <> ys.
+Proof.
+  intros H P.
+  apply H.
+  now rewrite P.
+Qed.
+
+Lemma prefix_extend A (xs ys:list A) a : xs<>ys++[a] -> prefix xs (ys ++ [a]) -> prefix xs ys.
+Proof.
+  revert ys; induction xs.
+  - easy.
+  - intros ys H P.
+    destruct (ys++[a]) eqn:eq; try easy.
+    simpl in P; destruct P as (E,P),E.
+    apply neq_extend in H.
+    destruct ys.
+    + simpl in eq.
+      assert (l=[]) as E.
+      * apply (@f_equal _ _ (@length _) [a] (a0::l)) in eq.
+        injection eq; intros E.
+        symmetry in E.
+        now apply length_zero_iff_nil in E.
+      * rewrite E in *.
+        now destruct xs.
+    + rewrite <- app_comm_cons in eq.
+      injection eq; intros H1 H2.
+      destruct H2.
+      rewrite <- H1 in *.
+      simpl; split; try easy.
+      now apply IHxs.
+Qed.
+
+Lemma prefix_propagate A (x y z:list A) : prefix x z -> prefix y z -> prefix x y \/ prefix y x.
+Proof.
+  revert y z.
+  induction x.
+  - intuition.
+  - intros y z XZ YZ.
+    destruct z,y; intuition; try easy.
+    destruct XZ as (E1,XZ), YZ as (E2,YZ).
+    assert (prefix x y \/ prefix y x) as H by (now apply IHx with z).
+    destruct H; [left | right]; rewrite E1, <- E2; now split.
+Qed.
+
+Definition noprefix A (xs ys:list A) := not (prefix xs ys) /\ not (prefix ys xs).
+
+Lemma noprefix_cons A (x y:A) (xs ys:list A) : x=y -> noprefix (x::xs) (y::ys) <-> noprefix xs ys.
+Proof. firstorder. Qed.
+
+Lemma noprefix_cons' A (x y:A) (xs ys:list A) : x<>y -> noprefix xs ys -> noprefix (x::xs) (y::ys).
+Proof. intros n; split; intros (H1,H2); congruence. Qed.
+
+Require Import Coq.Structures.Equalities.
+
+Module Dec(X:MiniDecidableType).
+  Module XX := Make_UDT(X).
+
+  Import X XX.
+
+  Lemma prefix_dec (xs ys:list t) : prefix xs ys \/ ~ prefix xs ys.
+  Proof.
+    revert ys.
+    induction xs; intros ys.
+    - now left.
+    - destruct ys.
+      + now right.
+      + destruct (eq_dec a t0).
+        * specialize IHxs with ys; destruct IHxs.
+          -- now left.
+          -- right; intros (H1,H2); congruence.
+        * right; intros (H1,H2); congruence.
+  Qed.
+
+  Lemma not_noprefix_prefix (xs ys : list t) : ~ noprefix xs ys -> prefix xs ys \/prefix ys xs.
+  Proof.
+    intros H.
+    destruct (prefix_dec xs ys).
+    - left; easy.
+    - destruct (prefix_dec ys xs).
+      + right; easy.
+      + exfalso; apply H; now split.
+  Qed.
+End Dec.
